Remove bexp/lexp syntax classes from GPUCSL

src/GPUCSL/Host.v
@@ -51,10 +51,10 @@ Record State := St {
   st_heap : simple_heap
 }.
 
-Fixpoint alloc_heap (start : nat) (vs : list Z) : simple_heap :=
+Fixpoint alloc_heap (start : nat) (vs : list val) : simple_heap :=
   match vs with
   | nil => fun x => None
-  | v :: vs => fun l => if Z.eq_dec l (Zn start) then Some (VZ v) else alloc_heap (S start) vs l
+  | v :: vs => fun l => if Z.eq_dec l (Zn start) then Some v else alloc_heap (S start) vs l
   end.
 
 Fixpoint bind_params (stk : stack) (xs : list var) (vs : list val) : Prop :=
@@ -108,7 +108,7 @@ Inductive stmt_step : GModule -> stmt -> State -> stmt -> State -> Prop :=
     edenote e (st_stack gst) = Some (VZ (Z.of_nat (length vs))) ->
     hdisj (st_heap gst) (alloc_heap start vs) ->
     stmt_step kenv (host_alloc x e) gst
-              host_skip (St (var_upd (st_stack gst) x (VZ (Z.of_nat start)))
+              host_skip (St (var_upd (st_stack gst) x (VPtr (GLoc (Z.of_nat start))))
                             (hplus (st_heap gst) (alloc_heap start vs)))
 | Exec_iLet kenv x e (gst : State) n :
     edenote e (st_stack gst) = Some n ->
@@ -472,20 +472,24 @@ Proof.
   intros Hint Hinst; induction Hinst; simpl in *; eauto.
 Qed.
 
-Lemma subst_ent_bind_params y v xs vs s :
-  subst_ent y v xs vs
-  -> bind_params s xs vs 
-  -> (s y = v).
+Definition vals_lvals_equiv vs lvs := List.Forall2 val_lval_equiv vs lvs.
+
+Lemma subst_ent_bind_params y lv xs vs lvs s :
+  subst_ent y lv xs lvs (* (y = x)[vs/xs] *)
+  -> bind_params s xs vs (* s(xs) = vs *)
+  -> vals_lvals_equiv vs lvs
+  -> val_lval_equiv (s y) lv.
 Proof.
-  revert vs; induction xs as [|x xs]; simpl; try tauto.
-  intros [|v' vs]; try tauto.
-  destruct var_eq_dec; substs; jauto.
-  intros ? [? ?]; eauto; substs; eauto.
+  revert vs lvs; induction xs as [|x xs]; simpl; try tauto.
+  intros [|v' vs] [|lv' lvs]; try tauto.
+  destruct var_eq_dec; intros ? Hbin Heq; substs; inverts Heq; jauto.
+  cutrewrite (s y = v'); tauto.
 Qed.
 
-Lemma subst_env_bind_params E xs vs s : 
-  subst_env E xs vs
+Lemma subst_env_bind_params E xs lvs vs s : 
+  subst_env E xs lvs
   -> bind_params s xs vs
+  -> vals_lvals_equiv vs lvs
   -> env_assns_denote E s.
 Proof.
   revert xs vs s; induction E as [| [y v'] E]; introv; simpl; eauto.
@@ -674,6 +678,30 @@ Proof.
   [do 3 eexists|do 2 eexists]; split; eauto.
 Qed.
 
+Lemma Forall2_In1 A B P (xs : list A) (ys : list B) x :
+  Forall2 P xs ys 
+  -> In x xs
+  -> exists y, In y ys /\ P x y.
+Proof.
+  revert ys; induction 1; simpl; try tauto.
+  intros [? | Hin]; substs.
+  - exists y; splits; eauto.
+  - forwards* (? & ? & ?): IHForall2.
+Qed.
+
+Lemma evalExpseq_ok s E es lvs :
+  env_assns_denote E s
+  -> evalExpseq E es lvs
+  -> exists vs, Forall2 (fun e v => edenote e s = Some v) es vs /\
+                Forall2 val_lval_equiv vs lvs.
+Proof.
+  induction 2; intros.
+  - exists (@nil val); split; constructor.
+  - forwards* (v & ? & ?): evalExp_ok.
+    destruct IHForall2 as [vs ?].
+    exists (v :: vs); split; constructor; jauto.
+Qed.
+
 Lemma rule_invk (G : FC) (fn : string) (nt nb : nat) (es : list exp)
       (vs : list lval)
       fs ent ntrd enb nblk
@@ -695,7 +723,7 @@ Lemma rule_invk (G : FC) (fn : string) (nt nb : nat) (es : list exp)
   -> CSLh G
             (Assn R P E)
             (host_invoke fn ent enb es)
-            (Assn RF P E ** Q 0%Z).
+            (Assn RF P E ** Q (VZ 0%Z)).
 Proof.
   intros Hfcok Htag Hinfn Harg Hinst HQvar Heval Hntrd Hnblk Hsubst Hp Hr n HFC s h Hsat.
   forwards*: (fc_ok_func_disp).
@@ -708,15 +736,21 @@ Proof.
   - inversion 1.
   - introv Hdisj Htoh Habort.
     inverts Habort as Hent0 Henb0 Habort.
+    { destruct Hsat as (? & ? & Henv).
+      forwards* (? & ? & ?): (>>evalExp_ok Hent).
+      forwards* (? & ? & ?): (>>evalExp_ok Henb).
+      destruct Hent0 as [? | [? | (e & Hin & ?)]]; try congruence.
+      forwards* (? & ? & Heval'): (>>Forall2_In1 Heval Hin); try congruence.
+      forwards* (? & ? & ?): (>>evalExp_ok Heval'); try congruence. }
     destruct Habort as [? | [ [? ?] | [Hn0 | [Hm0 | Hcallab] ]]]; try congruence.
     + unfold sat in Hsat; simpl in Hsat.
-      forwards* Hent': (>>evalExp_ok Hent).
-      hnf in Hent'; simpl in Hent'; substs.
-      rewrite Hent', Nat2Z.inj_iff in Hent0; eauto.
+      forwards* (? & ? & ?): (>>evalExp_ok Hent).
+      simpl in *; substs.
+      assert (Zn ntrd = Zn 0) by congruence; lia.
     + unfold sat in Hsat; simpl in Hsat. 
-      forwards* Henb': (>>evalExp_ok Henb).
-      hnf in Henb'; simpl in Henb'; substs.
-      rewrite Henb', Nat2Z.inj_iff in Henb0; eauto.
+      forwards* (? & ? & ?): (>>evalExp_ok Henb).
+      simpl in *; substs.
+      assert (Zn nblk = Zn 0) by congruence; lia.
     + forwards* Hc: (>> Hcallab Hdisp); simpl in Hc.
   - introv Hdis Htoh Hstep.
     simpl in HFC; rewrite <-minus_n_O in HFC.
@@ -733,27 +767,23 @@ Proof.
     forwards* (h1' & h2' & ? & ? & Heq12'): (>> phplus_gheap  Heq12); substs.
     assert (Heq : nb0 = nblk); [ | subst nb0 ].
     { unfold sat in Hsat; simpl in Hsat.
-      forwards* Henb'': (>>evalExp_ok Henb).
-      hnf in Henb''; simpl in Henb''; substs.
-      rewrite Henb'', Nat2Z.inj_iff in Henb'; eauto. }
+      forwards* (? & ? & ?): (>>evalExp_ok Henb); simpl in *; substs.
+      assert (Zn nb0 = Zn nblk) by congruence; lia. }
     assert (Heq : nt0 = ntrd); [ | subst nt0 ].
     { unfold sat in Hsat; simpl in Hsat.
-      forwards* Hent'': (>>evalExp_ok Hent).
-      hnf in Hent''; simpl in Hent''; substs.
-      rewrite Hent'', Nat2Z.inj_iff in Hent'; substs; eauto. }
+      forwards* (? & ? & ?): (>>evalExp_ok Hent); simpl in *; substs.
+      assert (Zn nt0 = Zn ntrd) by congruence; lia. }
     forwards* Hsafe: (>>Hfn' h1' Hinit Hbnd).
     (* Proof that precond holds *)
     { unfold sat; simpl; splits; jauto.
       forwards*Henv: Hsubst.
-      applys* (>>subst_env_bind_params Henv).
+      applys* (>>subst_env_bind_params (VZ (Zn nblk) :: VZ (Zn ntrd) :: vs0) Henv).
       repeat split; eauto using initGPU_ntrd, initGPU_nblk.
-      simpl in Hsubst.
-      cutrewrite (vs = vs0); eauto.
-      destruct Hsat as (_ & _ & HP).
-      revert Heval Heval' HP; clear.
-      intros H; revert vs0; induction H; inversion 1; intros; substs; eauto.
-      forwards*: evalExp_ok.
-      f_equal; eauto. }
+      repeat constructor.
+      forwards* (vs' & Hevales & Heq): evalExpseq_ok.      
+      cutrewrite (vs0 = vs'); eauto.
+      generalize Heval' vs' Hevales; clear; induction 1; intros ? Heval; inverts Heval; eauto.
+      forwards*: IHHeval'; substs; congruence. }
     (* h **                                     hF -> 
        h1' ** (h2' : framed w.r.t. fun exec. ) ** hF -> *)
     exists h; splits; eauto.
@@ -769,8 +799,8 @@ Lemma safe_nh_exec_hfun n s (h1 h2 : zpheap) (disj : pdisj h1 h2) body ret x s_r
   -> sat_res (as_gheap h2) R 
   -> env_assns_denote E s_ret
   -> (forall v, has_no_vars (Q v))
-  -> safe_nh n s (@phplus_pheap val h1 h2 disj) (host_exec_hfun body ret x s_ret)
-             (Ex v, Assn R P (x |-> v :: (remove_var E x)) ** Q v).
+  -> safe_nh n s (phplus_pheap disj) (host_exec_hfun body ret x s_ret)
+             (Ex v, Assn R P (x |-> Vval v :: (remove_var E x)) ** Q v).
 Proof.
   revert s h1 h2 disj body; induction n; simpl; introv; eauto.
   intros (Hskip & Hsafe & Hstep) HP Hres Henv Qinde; splits; eauto.
@@ -801,7 +831,7 @@ Proof.
         forwards* Hsat: Hskip.
         exists (s ret).
         exists (as_gheap h2) (as_gheap h1); splits; jauto; fold_sat.
-        -- splits; simpl; jauto.
+        -- splits; simpl; unfold ent_assn_denote; simpl; jauto.
            splits; [unfold var_upd; destruct var_eq_dec; congruence|].
            applys* (>>disjoint_inde_env (x :: nil)); simpl; eauto.
            ++ apply remove_var_inde.
@@ -834,7 +864,7 @@ Lemma rule_call (G : FC) x (fn : string) (es : list exp)
   -> CSLh G
             (Assn R P E)
             (host_call x fn es)
-            (Ex v, Assn RF P (x |-> v :: (remove_var E x)) ** Q v).
+            (Ex v, Assn RF P (x |-> Vval v :: (remove_var E x)) ** Q v).
 Proof.
   intros Hfcok Htag Hinfn Harg Hinst HQinde Heval Hsubst Hp Hr n HFC s h Hsat.
   destruct n; simpl; eauto.
@@ -845,6 +875,10 @@ Proof.
   - inversion 1.
   - introv Hdisj Htoh Habort.
     inverts Habort as Habort.
+    { destruct Hsat as (? & ? & Henv).
+      destruct Habort as (e & Hin & ?); try congruence.
+      forwards* (? & ? & Heval'): (>>Forall2_In1 Heval Hin); try congruence.
+      forwards* (? & ? & ?): (>>evalExp_ok Heval'); try congruence. }
     destruct Habort as [? | [ [? ?] | Hcallab] ]; try congruence.
     forwards* Hc: (>> Hcallab Hdisp); simpl in Hc.
   - introv Hdis Htoh Hstep.
@@ -864,12 +898,10 @@ Proof.
     (* Proof that precond holds *)
     { unfold sat; splits; jauto.
       applys* subst_env_bind_params.
-      cutrewrite (vs = vs0); eauto.
-      destruct Hsat as (_ & _ & HP).
-      revert Heval Heval' HP; clear.
-      intros H; revert vs0; induction H; inversion 1; intros; substs; eauto.
-      forwards*: evalExp_ok.
-      f_equal; eauto. }
+      forwards* (vs' & Hevales & Heq): evalExpseq_ok.
+      cutrewrite (vs0 = vs'); eauto.
+      generalize Heval' vs' Hevales; clear; induction 1; intros ? Heval; inverts Heval; eauto.
+      forwards*: IHHeval'; substs; congruence. }
     (* h **                                     hF -> 
        h1' ** (h2' : framed w.r.t. fun exec. ) ** hF -> *)
     exists h; splits; eauto.
@@ -904,14 +936,16 @@ Proof.
   intros Heval n _ s h Hsat; destruct n; simpl; eauto; splits. 
   - inversion 1.
   - introv Hdis Heq Hc; inverts Hc.
+    hnf in Hsat; forwards* (? & ? & ?): evalExp_ok; congruence.
   - introv Hdis Heq Hstep.
     inverts Hstep.
     exists h; splits; eauto.
     apply safe_nh_skip.
     unfold sat in Hsat |- *; simpl in Hsat.
     simpl; splits; jauto.
-    + unfold var_upd; destruct var_eq_dec; try congruence.
-      forwards*: evalExp_ok.
+    + forwards* (? & ? & ?): evalExp_ok.
+      unfold var_upd; destruct var_eq_dec; try congruence.
+      simpl in *; cutrewrite (n0 = x0); [eauto|congruence].
     + applys* (>>disjoint_inde_env (x :: nil)); simpl; eauto.
       apply remove_var_inde; simpl; eauto.
       applys* remove_var_imp.
@@ -974,20 +1008,21 @@ Proof.
 Qed.
 
 Lemma rule_host_alloc G R P E x e size : 
-  evalExp E e (Zn size)
+  evalExp E e (Vval (VZ (Zn size)))
   -> CSLh G (Assn R P E)
             (host_alloc x e)
-            (Ex p vs, Assn (array (GLoc p) vs 1 *** R) (length vs = size /\ P) ((x |-> p) :: (remove_var E x))).
+            (Ex p vs, Assn (array p vs 1 *** R) (length vs = size /\ P) ((x |-> Vval (VPtr p)) :: (remove_var E x))).
 Proof.
   intros Heval n _ s h Hsat; destruct n; simpl; eauto; splits. 
   - inversion 1.
   - introv Hdis Heq Hc; inverts Hc.
+    hnf in Hsat; forwards* (? & ? & ?): evalExp_ok; congruence.
   - introv Hdis Heq Hstep.
     inverts Hstep as Heval' Hdis'; simpl in *.
     unfold sat in Hsat; simpl in Hsat.
-    forwards* Heval'': evalExp_ok; simpl in Heval''.
+    forwards* (v & Heval'' & ?): evalExp_ok; simpl in Heval''.
     assert (size = length vs); [|subst size].
-    { rewrite Heval'' in Heval'; rewrite Nat2Z.inj_iff in Heval'; eauto. }
+    { assert (Zn (length vs) = Zn size) by congruence; lia. }
     pose (htop (alloc_heap start vs)) as h_alc.
     forwards* Heq': ptoheap_eq.
     lets Hdis_alc: Hdis'.
@@ -1006,7 +1041,7 @@ Proof.
       apply ptoheap_plus; eauto using hdisjC.
       apply ptoheap_htop.
     + apply safe_nh_skip.
-      exists (Zn start) vs.
+      exists (GLoc (Zn start)) vs.
       unfold sat in Hsat |- *; simpl in Hsat.
       simpl; splits; jauto.
       -- exists (as_gheap h_alc) (as_gheap h); splits; jauto.
@@ -1113,4 +1148,3 @@ End Rules.
 
 Notation "'All' x .. y ',' tri" := (FAll _ (fun x => .. (FAll _ (fun y => tri)) ..))
                                      (at level 200, x binder, y binder, tri at level 200).
-
