src/GPUCSL/GPUCSL.v
@@ -9,14 +9,18 @@ Require Import MyVector.
 Definition default ntrd : (Vector.t assn ntrd * Vector.t assn ntrd) := 
   (init (fun _ => Emp_assn), init (fun _ => Emp_assn)).
 
-Infix "+C" := (Ebinop OP_plus) (at level 50, left associativity).
-Infix "*C" := (Ebinop OP_mult) (at level 40, left associativity).
-Infix "-C" := (Ebinop OP_sub) (at level 50, left associativity).
-Infix "<C" := (Bcomp OP_blt) (at level 55).
-Infix "==C" := (Bcomp OP_beq) (at level 55).
-Infix "/C" := (Ebinop OP_div) (at level 40, left associativity).
-Infix "%C" := (Ebinop OP_mod) (at level 40, left associativity).
-Infix "&&C" := (Bbool OP_and) (at level 56, left associativity).
-Infix "||C" := (Bbool OP_or) (at level 57, left associativity).
-Notation minC x y := (Ebinop OP_min x y).
+Infix "+C" := (Ebinop (OP_arith OP_plus)) (at level 50, left associativity).
+Infix "*C" := (Ebinop (OP_arith OP_mult)) (at level 40, left associativity).
+Infix "-C" := (Ebinop (OP_arith OP_sub)) (at level 50, left associativity).
+Infix "<C" := (Ebinop (OP_comp OP_lt)) (at level 55).
+Infix "==C" := (Ebinop (OP_comp OP_eq)) (at level 55).
+Infix "/C" := (Ebinop (OP_arith OP_div)) (at level 40, left associativity).
+Infix "%C" := (Ebinop (OP_arith OP_mod)) (at level 40, left associativity).
+Infix "&&C" := (Ebinop (OP_bool OP_and)) (at level 56, left associativity).
+Infix "||C" := (Ebinop (OP_bool OP_or)) (at level 57, left associativity).
+Notation minC x y := (Ebinop (OP_arith OP_min) x y).
 Notation Zn := Z.of_nat.
+
+Coercion VZ : Z >-> val.
+Coercion VPtr : loc >-> val.
+Coercion Vval : val >-> lval.
